io/ho_examples/Callback.Level2.fst
@@ -49,7 +49,7 @@ assume val pi : monitorable_prop
 
 (** the problem I suspected exists. **)
 
-assume val ctx_cb_post_monitorable : monitorable_hist ctx_cb_pre ctx_cb_post pi
+assume val ctx_cb_post_monitorable : checkable_hist_post ctx_cb_pre ctx_cb_post pi
 
 let ctx_cb_instrumentable : instrumentable ctx_cb pi =
   instrumentable_IIO_strengthen
@@ -58,23 +58,35 @@ let ctx_cb_instrumentable : instrumentable ctx_cb pi =
     ctx_cb_pre ctx_cb_post pi #ctx_cb_post_monitorable
 
 assume val pp_cb_pre_checkable : checkable pp_cb_pre
-assume val pp_cb_post_cpi : squash (forall h lt r. pp_cb_pre h /\ pp_cb_post h r lt ==> enforced_locally pi h lt)
+assume val pp_cb_monitorable_hist : monitorable_hist #ctx_cb (fun _ -> pp_cb_pre) (fun _ -> pp_cb_post) pi 
  
 let pp_cb_mlifyable_in : mlifyable_in_arr0 ctx_cb pp_cb_out pp_cb_pre pp_cb_post pi = {
-  cmlifyable0 = mlifyable_inst_iiowp_trivialize_weaken ctx_cb #ctx_cb_instrumentable pp_cb_out #pp_cb_out_exportable pp_cb_pre #pp_cb_pre_checkable pp_cb_post;
-  cpi0 = pp_cb_post_cpi;
+  cmlifyable0 =
+    mlifyable_inst_iiowp_trivialize_weaken'
+      ctx_cb #ctx_cb_instrumentable
+      pp_cb_out #pp_cb_out_exportable
+      pp_cb_pre #pp_cb_pre_checkable
+      pp_cb_post
+      #pp_cb_monitorable_hist;
   ca0 = ctx_cb_instrumentable;
 }
 
-assume val ctx_post_monitorable : monitorable_hist #pp_cb_mlifyable_in.cmlifyable0.matype (fun x -> ctx_pre) (fun x -> ctx_post) pi
+assume val ctx_post_monitorable : checkable_hist_post #pp_cb_mlifyable_in.cmlifyable0.matype (fun x -> ctx_pre) (fun x -> ctx_post) pi
 
 let ctx_instrumentable : instrumentable ctx pi =
-  instrumentable_HO_arr0_out_importable ctx_cb pp_cb_out pp_cb_pre pp_cb_post ctx_out ctx_pre ctx_post pi
-  #ctx_out_importable
-  #pp_cb_mlifyable_in
-  #ctx_post_monitorable
+  instrumentable_HO_arr0_out_importable
+    ctx_cb pp_cb_out pp_cb_pre pp_cb_post
+    ctx_out ctx_pre ctx_post
+    pi
+    #ctx_out_importable
+    #pp_cb_mlifyable_in
+    #ctx_post_monitorable
   
 assume val pp_pre_checkable : checkable pp_pre
 
-let pp_mlifyable : mlifyable pp =
-  mlifyable_inst_iiowp_trivialize_weaken ctx #ctx_instrumentable pp_out #pp_out_exportable pp_pre #pp_pre_checkable pp_post 
+let pp_mlifyable : mlifyable pp (trivial_pi ())=
+  mlifyable_inst_iiowp_trivialize_weaken
+    ctx #ctx_instrumentable
+    pp_out #pp_out_exportable
+    pp_pre #pp_pre_checkable
+    pp_post 
